WIP
WIP

WIP

WIP

WIP

WIP

WIP

Debugging

WIP

WIP

WIP

WIP

WIP

WIP

WIP

WIP

WIP

WIP

WIP

WIP

WIP

WIP

WIP

WIP

WIP

WIP

WIP

WIP

WIP

WIP

WIP

WIP

Add bound_op

WIP

WIP

WIP

copy_bounds, fill_template

WIP

WIP

WIP

Fix bugs in shr

WIP

WIP

copy_bounds, fill_templates

Add LadderStepDisplay

copy_bounds

Add more notations

Copy bounds

Fix bounds

More notations

C code

More notations for fewer casts

Update log, fix shr

Don't insert identity casts

Update log with elimination of identity casts

Remove useless + casts

Remove useless & casts

Update 32-bit ladder step

Various small notation fixes

Add print of 32-bit ladder

Fix binary notation in 32-bit

Update notations

Update MulDisplay

Add display target

Update notations import

Update notations import

Update display target

Add a bunch of C display files

Remove lowercase files

Add MapBounds

Add 41417 MulDisplay

WIP

Add ComputeBounds

WIP

More/better C notations

Some binary things, remove extra notation

Add Java notations

Remove Java

Hopefully better java display targets

Add Java display things

Add more java display

Add src/SpecificGen/GF25519_64Reflective/Reified/LadderStepJavaDisplay.log

Add more java logs

Constant notation fixes

Add comment about Java casts

davidben tells me unsigned short is bigger than uint8_t

More notations fixes

Fix constants in display

Add more java display

Update display

WIP

WIP

Add TODO

Update TODO

Add to TODO

WIP on good bounds

WIP on good bounds

WIP on good bounds

WIP

WIP

WIP

WIP

Add Z.log2_up_nonneg to zarith

Add valid_update lemmas about FixedWordSizes

WIP

src/Reflection/Z/Syntax/Util.v
@@ -2,6 +2,23 @@ Require Import Crypto.Reflection.Syntax.
 Require Import Crypto.Reflection.Z.Syntax.
 
 Definition make_const t : interp_base_type t -> op Unit (Tbase t)
-  := match t with TZ => OpConst end.
+  := OpConst.
 Definition is_const s d (v : op s d) : bool
-  := match v with OpConst _ => true | _ => false end.
+  := match v with OpConst _ _ => true | _ => false end.
+Arguments is_const [s d] v.
+Definition is_cast s d (v : op s d) : bool
+  := match v with Cast _ _ => true | _ => false end.
+Arguments is_cast [s d] v.
+
+Definition base_type_max (v1 v2 : base_type) : base_type
+  := match v1, v2 with
+     | TZ, _ => TZ
+     | _, TZ => TZ
+     | TWord logsz1, TWord logsz2 => TWord (max logsz1 logsz2)
+     end.
+Definition base_type_min (v1 v2 : base_type) : base_type
+  := match v1, v2 with
+     | TZ, v => v
+     | v, TZ => v
+     | TWord logsz1, TWord logsz2 => TWord (min logsz1 logsz2)
+     end.
