src/Specific/GF25519Reflective/CommonBinOp.v
@@ -3,14 +3,13 @@ Require Import Crypto.Specific.GF25519BoundedCommon.
 Require Import Crypto.Reflection.Z.Interpretations64.
 Require Import Crypto.Reflection.Syntax.
 Require Import Crypto.Reflection.SmartMap.
-Require Import Crypto.Reflection.Application.
 Require Import Crypto.Util.Tactics.
 
 Local Opaque Interp.
 Lemma ExprBinOp_correct_and_bounded
-      ropW op (ropZ_sig : rexpr_binop_sig op)
-      (Hbounds : correct_and_bounded_genT ropW ropZ_sig)
-      (H0 : forall xy
+      ropZ op (ropZ_sig : rexpr_binop_sig op)
+      (Hbounds : correct_and_bounded_genT ropZ ropZ_sig)
+      (*(H0 : forall xy
                    (xy := (eta_fe25519W (fst xy), eta_fe25519W (snd xy)))
                    (Hxy : is_bounded (fe25519WToZ (fst xy)) = true
                           /\ is_bounded (fe25519WToZ (snd xy)) = true),
@@ -37,10 +36,36 @@ Lemma ExprBinOp_correct_and_bounded
           with
           | Some bounds => binop_bounds_good bounds = true
           | None => False
-          end)
-  : binop_correct_and_bounded ropW op.
+          end)*)
+  : binop_correct_and_bounded ropZ op.
 Proof.
-  intros x y Hx Hy.
+  intros xy HxHy.
+  cbv zeta in Hbounds.
+  destruct_head' and.
+  subst; rewrite <- (proj2_sig ropZ_sig).
+  unfold Relations.related_wordW, Relations.related_bounds, Relations.related_Z in *.
+  eapply LiftOption.lift_relation_type_pointwise in H0.
+  eapply LiftOption.lift_relation_type_pointwise in H2.
+  eapply LiftOption.lift_relation2_type_pointwise in H1.
+  { setoid_rewrite Relations.lift_interp_type_rel_pointwise_f_eq_id2 in H0.
+    setoid_rewrite Relations.lift_interp_type_rel_pointwise_f_eq_id2 in H2.
+    setoid_rewrite Relations.lift_interp_type_rel_pointwise_f_eq_id2 in H1.
+    cbv [ExprBinOpT] in *.
+    simpl @interp_flat_type in *.
+    specialize (H0 xy).
+
+  unfold Relations.related'_Z in *.
+  unfold Relations.proj_eq_rel in *.
+  Locate LiftOption.lift_relation.
+
+  Check LiftOption.of'.
+  unfold interp_type_rel_pointwise, interp_type_gen_rel_pointwise, interp_type_gen_rel_pointwise_hetero, ExprBinOpT, Morphisms.respectful_hetero, interp_flat_type_rel_pointwise, interp_flat_type_rel_pointwise_gen_Prop in *.
+  simpl @interp_flat_type in *.
+  cbv
+
+  simpl in x, y, Hx, Hy.
+
+  simpl in HxHy.
   pose x as x'; pose y as y'.
   hnf in x, y; destruct_head' prod.
   specialize (H0 (x', y') (conj Hx Hy)).
