src/Specific/GF25519Reflective/Reified/PreFreeze.v
@@ -1,17 +1,16 @@
-Require Import Crypto.Specific.GF25519Reflective.CommonUnOp.
+Require Import Crypto.Specific.GF25519Reflective.Common.
 
-Definition rprefreezeZ_sig : rexpr_unop_sig prefreeze. Proof. cbv [prefreeze GF25519.prefreeze]. reify_sig. Defined.
-Definition rprefreezeW := Eval vm_compute in rword_of_Z rprefreezeZ_sig.
-Lemma rprefreezeW_correct_and_bounded_gen : correct_and_bounded_genT rprefreezeW rprefreezeZ_sig.
-Proof. rexpr_correct. Qed.
-Definition rprefreeze_output_bounds := Eval vm_compute in compute_bounds rprefreezeW ExprUnOp_bounds.
+Definition rprefreezeZ_sig : rexpr_unop_sig prefreeze. Proof. reify_sig. Defined.
+Definition rprefreezeZ : Syntax.Expr _ _ _ := Eval vm_compute in proj1_sig rprefreezeZ_sig.
+Definition rprefreezeW : Syntax.Expr _ _ _ := Eval vm_compute in rexpr_select_word_sizes rprefreezeZ ExprUnOp_bounds.
+Definition rprefreezeZ_Wf : rexpr_wfT rprefreezeZ. Proof. prove_rexpr_wfT. Qed.
+Definition rprefreeze_output_bounds
+  := Eval vm_compute in compute_bounds rprefreezeZ ExprUnOp_bounds.
 Local Obligation Tactic := intros; vm_compute; constructor.
-Program Definition rprefreezeW_correct_and_bounded
-  := ExprUnOp_correct_and_bounded
-       rprefreezeW prefreeze rprefreezeZ_sig rprefreezeW_correct_and_bounded_gen
-       _ _.
+Program Definition rprefreezeZ_correct_and_bounded
+  := rexpr_correct_and_bounded rprefreezeZ rprefreezeZ_Wf ExprUnOp_bounds.
 
 Local Open Scope string_scope.
-Compute ("PreFreeze", compute_bounds_for_display rprefreezeW ExprUnOp_bounds).
-Compute ("PreFreeze overflows? ", sanity_compute rprefreezeW ExprUnOp_bounds).
-Compute ("PreFreeze overflows (error if it does)? ", sanity_check rprefreezeW ExprUnOp_bounds).
+Compute ("PreFreeze", compute_bounds_for_display rprefreezeZ ExprUnOp_bounds).
+Compute ("PreFreeze overflows? ", sanity_compute rprefreezeZ ExprUnOp_bounds).
+Compute ("PreFreeze overflows (error if it does)? ", sanity_check rprefreezeZ ExprUnOp_bounds).
